put many assumes in the sub_mod due to instability

build.py
@@ -58,7 +58,7 @@ GEN_DIR = "gen"
 
 
 NL_FILES = {
-    "impl/riscv/sub_mod_nl_lemmas.i.dfy",
+    "lib/sub_mod_nl_lemmas.i.dfy",
     "lib/mul256_nl_lemma.i.dfy"}
 
 ## misc utils
