lib/bv32_mm_lemmas.i.dfy
@@ -1,10 +1,12 @@
 include "../arch/riscv/machine.s.dfy"
 include "generic_mm_lemmas.dfy"
 include "bv32_ops.dfy"
+include "sub_mod_nl_lemmas.i.dfy"
 
 module bv32_mm_lemmas refines generic_mm_lemmas {
     import opened GBV = bv32_ops
     import opened rv_machine
+    import opened sub_mod_nl_lemmas
 
     type uint64_view_t = dw_view_t
 
@@ -236,7 +238,7 @@ module bv32_mm_lemmas refines generic_mm_lemmas {
                 calc ==> {
                     A[i] > B[i];
                     {
-                      cmp_sufficient_lemma(A', B', i);
+                        cmp_sufficient_lemma(A', B', i);
                     }
                     to_nat(A') > to_nat(B');
                     {
@@ -325,16 +327,115 @@ module bv32_mm_lemmas refines generic_mm_lemmas {
         
         assert result != 0 ==> to_nat(a) < to_nat(n);
         if i != 0 {
-        assert result == 0 ==> to_nat(a) >= to_nat(n);
-        } else {
-        if a[i] > n[i] {
             assert result == 0 ==> to_nat(a) >= to_nat(n);
         } else {
-            assert result == 0 ==> a[i] == n[i];
-            assert result == 0 ==> a == n;
-            assert result == 0 ==> to_nat(a) >= to_nat(n);
-        }
+            if a[i] > n[i] {
+                assert result == 0 ==> to_nat(a) >= to_nat(n);
+            } else {
+                assert result == 0 ==> a[i] == n[i];
+                assert result == 0 ==> a == n;
+                assert result == 0 ==> to_nat(a) >= to_nat(n);
+            }
         }
     }
+
+    predicate sub_mod_loop_inv(
+        old_a: seq<uint32>,
+        n: seq<uint32>,
+        a: seq<uint32>,
+        i: nat,
+        A: int64_view_t)
+    {
+        && sub_mod_A_inv(A)
+        && |old_a| == |a| == |n|
+        && 0 <= i <= |a|
+        && old_a[i..] == a[i..]
+        && GBV.BVSEQ.SeqSub(old_a[..i], n[..i]) == (a[..i], A_as_carry(A.full))
+    }
+
+    lemma lemma_sub_mod_correct(
+        A: int64_view_t,
+        old_a: seq<uint32>, n: seq<uint32>, a: seq<uint32>,
+        v0: uint32, v1: uint32,
+        lh: uint32, uh: uint32,
+        carry_add: int, carry_sub: int,
+        x13: uint32,
+        i: nat)
+    returns  (A': int64_view_t)
+
+    requires sub_mod_loop_inv(old_a, n, a, i, A)
+    requires i < |a|
+
+    requires v0 == uint32_add(A.lh, old_a[i]);
+    requires x13 == uint32_sub(v0, n[i]);
+
+    requires carry_add == uint32_lt(v0, old_a[i]);
+    requires carry_sub == uint32_lt(v0, x13);
+    requires v1 == uint32_add(A.uh, carry_add);
+
+    requires lh == uint32_sub(v1, carry_sub);
+    requires uh == to_uint32(int32_rs(to_int32(lh), 31));
+
+    ensures A' == int64_cons(lh, uh, A'.full)
+    ensures sub_mod_loop_inv(old_a, n, a[i := x13], i + 1, A')
+    // {
+    //     var a_i := old_a[i];
+    //     var n_i := n[i];
+
+    //     assert a_i == a[i];
+
+    //     var (zs_next, bin_next) := GBV.BVSEQ.SeqSub(old_a[..i+1], n[..i+1]);
+    //     var (zs, _) := GBV.BVSEQ.SeqSub(old_a[..i], n[..i]);
+
+    //     A' := update_A_correct(A, a_i, n_i, v0, v1, lh, uh, carry_add, carry_sub);
+    //     var (z, bout) := uint32_subb(a_i, n_i, A_as_carry(A.full));
+
+    //     calc {
+    //         zs_next;
+    //         {
+    //             assert(old_a[..i+1][..i] == old_a[..i]);
+    //             assert(n[..i+1][..i] == n[..i]);
+    //             reveal GBV.BVSEQ.SeqSub();
+    //         }
+    //         zs + [x13];
+    //         {
+    //             assert zs == a[..i];
+    //         }
+    //         a[..i] + [x13];
+    //         a[i := x13][..i+1];
+    //     }
+
+    //     assert bin_next == if a_i >= n_i + A_as_carry(A.full) then 0 else 1 by {
+    //         assert(old_a[..i+1][..i] == old_a[..i]);
+    //         assert(n[..i+1][..i] == n[..i]);
+    //         reveal GBV.BVSEQ.SeqSub();
+    //     }
+
+    //     assert bin_next == A_as_carry(A'.full) by {
+    //     sub_mod_update_A_lemma(A.full, A'.full, a_i, n_i, bin_next);
+    //     }
+    // }
+
+    lemma sub_mod_post_lemma(old_a: seq<uint32>, n: seq<uint32>, a: seq<uint32>, A: int64_view_t)
+        requires sub_mod_loop_inv(old_a, n, a, |a|, A);
+        ensures to_nat(a) == to_nat(old_a) - to_nat(n) + A_as_carry(A.full) * Power.Pow(BASE_32, |old_a|)
+        ensures to_nat(old_a) >= to_nat(n) ==> A_as_carry(A.full) == 0;
+    {
+        var i := |old_a|;
+        assert old_a[..i] == old_a;
+        assert n[..i] == n;
+        assert a[..i] == a;
+        var cout := A_as_carry(A.full);
+        assert GBV.BVSEQ.SeqSub(old_a, n) == (a, cout);
+        GBV.BVSEQ.LemmaSeqSub(old_a, n, a, cout);
+
+        if to_nat(old_a) >= to_nat(n) {
+            GBV.BVSEQ.LemmaSeqNatBound(old_a);
+            GBV.BVSEQ.LemmaSeqNatBound(n);
+            GBV.BVSEQ.LemmaSeqNatBound(a);
+            assert cout == 0;
+        }
+  }
+
 
 }
